src/rocq/Theory/I2F/I2F_memory.v
@@ -1,0 +1,1119 @@
+From Equations Require Import Equations.
+
+From Stdlib Require Import
+  ZArith
+  Strings.String
+  List
+  Morphisms.
+Import ListNotations.
+
+From ITree Require Import Basics.HeterogeneousRelations.
+
+From Vellvm Require Import
+  Utils
+  Syntax
+  Semantics
+  VellvmIntegers
+  Integers
+  Interfaces.IPtr
+  Interfaces.Params
+  Interfaces.Pointer
+  Implementations.Pointer
+  Implementations.Provenance
+  Implementations.IPtrInfinite
+  Implementations.IPtrFinite
+  Implementations.Memory
+  Implementations.ParamsV
+  Interfaces.Memory.
+
+From Vellvm Require Import
+  Handlers.Memory.
+
+From Vellvm Require Import
+  Theory.I2F.Refinement
+  Theory.I2F.I2F_exp
+  Theory.I2F.I2F_MemS.
+
+Existing Instance MemoryModelStateV.
+Existing Instance MemoryModelPrimitivesV.
+
+(** * Relating [ptr]/[EOU] operations underlying the memory model
+
+    Pure facts about pointers and [EOU]-valued primitives (address
+    creation, sequences of intptrs, integer coercions) that the state-ful
+    lemmas below build on. *)
+
+Lemma I2F_Addr_ptr_to_int : forall (p : @ptr (@PROV PInf) (@PTR PInf)) (p' : @ptr (@PROV PFin) (@PTR PFin)),
+    I2F_Addr p p' -> @ptr_to_int _ _ (@P2I PInf) p = @ptr_to_int _ _ (@P2I PFin) p'.
+Proof.
+  intros [z pr] [i pr'] [HI ->]; cbn; red in HI; auto.
+Qed.
+
+Lemma I2F_Addr_ptr_provenance : forall p p',
+    I2F_Addr p p' -> ptr_provenance p = ptr_provenance p'.
+Proof.
+  intros [z pr] [i pr'] [HI ->]; cbn; auto.
+Qed.
+
+Lemma I2F_from_Z : forall z, I2F_EOU I2F_Iptr (@from_Z IPZ z) (@from_Z IP64Bit z).
+Proof.
+  intros z; cbn; unfold from_Z_bits.
+  destruct ((z <=? @Integers.max_unsigned 64) && (z >=? 0))%Z eqn:RANGE.
+  - constructor.
+    red.
+    apply andb_prop in RANGE as [LE GE].
+    apply Z.leb_le in LE; apply Z.geb_le in GE.
+    symmetry; apply Integers.unsigned_repr.
+    unfold Integers.max_unsigned in *; lia.
+  - constructor.
+Qed.
+
+Lemma I2F_int_to_ptr : forall z pr,
+    I2F_EOU I2F_Addr (@int_to_ptr _ _ (@PIV IPZ) z pr) (@int_to_ptr _ _ (@PIV IP64Bit) z pr).
+Proof.
+  intros z pr.
+  eapply I2F_EOU_bind; [apply I2F_from_Z |].
+  intros a1 a2 Ha; constructor; auto.
+Qed.
+
+(** [intptr_seq] traverses the SAME (Params-independent) index list on
+    both sides: a single-list [map_monad] compatibility suffices. *)
+Lemma I2F_intptr_seq : forall start size,
+    I2F_EOU (Forall2 I2F_Iptr) (@intptr_seq IPZ start size) (@intptr_seq IP64Bit start size).
+Proof.
+  intros start size; unfold intptr_seq.
+  apply I2F_EOU_map_monad.
+  intros a _; apply I2F_from_Z.
+Qed.
+
+Lemma I2F_get_consecutive_ptrs : forall p p',
+    I2F_Addr p p' ->
+    forall n,
+      I2F_EOU (Forall2 I2F_Addr)
+        (@get_consecutive_ptrs PInf p n)
+        (@get_consecutive_ptrs PFin p' n).
+Proof.
+  intros p p' Hp n; unfold get_consecutive_ptrs.
+  eapply I2F_EOU_bind; [apply I2F_intptr_seq |].
+  intros ixs1 ixs2 HIXS.
+  eapply I2F_EOU_map_monad_acc2; eauto.
+  intros ix1 ix2 Hix.
+  apply I2F_handle_gep_ptr; auto.
+Qed.
+
+Lemma I2F_coerce_integer_to_int : forall b z,
+    I2F_EOU I2F_dvalue_base (@coerce_integer_to_int PInf b z) (@coerce_integer_to_int PFin b z).
+Proof.
+  intros [sz|] z; unfold coerce_integer_to_int.
+  - repeat constructor.
+  - eapply I2F_EOU_bind; [apply I2F_from_Z |].
+    intros i1 i2 Hi; repeat constructor; auto.
+Qed.
+
+Lemma I2F_no_overlap : forall (a1 a2 : @ptr (@PROV PInf) (@PTR PInf)) sz1
+                              (a1' a2' : @ptr (@PROV PFin) (@PTR PFin)) sz2,
+    I2F_Addr a1 a1' -> I2F_Addr a2 a2' ->
+    @no_overlap _ _ (@overlaps_ptoi _ _ (@P2I PInf)) a1 sz1 a2 sz2 =
+    @no_overlap _ _ (@overlaps_ptoi _ _ (@P2I PFin)) a1' sz1 a2' sz2.
+Proof.
+  intros [z1 pr1] [z2 pr2] sz1 [i1 pr1'] [i2 pr2'] sz2 [HI1 ->] [HI2 ->].
+  red in HI1, HI2; subst.
+  reflexivity.
+Qed.
+
+Lemma I2F_mbyte_MByte : forall dv dv' dt idx,
+    I2F_dvalue dv dv' -> I2F_mbyte (MByte dv dt idx) (MByte dv' dt idx).
+Proof.
+  intros dv dv' dt idx H; red; cbn.
+  now apply I2F_dvalue_extract_byte.
+Qed.
+
+(** [generate_num_poison_bytes_h] is defined via [N.recursion] threading a
+    start index; unfold it one step at a time via the library's
+    [recursion_0]/[recursion_succ] equations (properness in the
+    accumulator is literal Leibniz equality here, so it is trivial) rather
+    than fighting the low-level fixpoint. *)
+Lemma generate_num_poison_bytes_h_0 {Pa : Params} (dt : dtyp) (start : N) :
+  generate_num_poison_bytes_h start 0 dt = [].
+Proof. reflexivity. Qed.
+
+Lemma generate_num_poison_bytes_h_succ {Pa : Params} (dt : dtyp) (start num : N) :
+  generate_num_poison_bytes_h start (N.succ num) dt =
+  MByte (DVALUE_Poison dt) dt start :: generate_num_poison_bytes_h (N.succ start) num dt.
+Proof.
+  unfold generate_num_poison_bytes_h.
+  assert (PROP : Proper (Logic.eq ==> Logic.eq ==> Logic.eq)
+            (fun (n : N) (mf : N -> list memory_byte) (x : N) =>
+               MByte (DVALUE_Poison dt) dt x :: mf (N.succ x))).
+  { intros n1 n2 -> mf1 mf2 ->; reflexivity. }
+  pose proof
+    (N.recursion_succ Logic.eq (fun _ : N => ([] : list memory_byte))
+       (fun n mf x => MByte (DVALUE_Poison dt) dt x :: mf (N.succ x))
+       eq_refl PROP num) as REC.
+  rewrite REC; cbn; reflexivity.
+Qed.
+
+Lemma I2F_generate_num_poison_bytes_h : forall start num dt,
+    Forall2 I2F_mbyte
+      (@generate_num_poison_bytes_h PInf start num dt)
+      (@generate_num_poison_bytes_h PFin start num dt).
+Proof.
+  intros start num; revert start; induction num using N.peano_ind; intros start dt.
+  - rewrite 2 generate_num_poison_bytes_h_0; constructor.
+  - rewrite 2 generate_num_poison_bytes_h_succ.
+    constructor; auto.
+    apply I2F_mbyte_MByte; repeat constructor.
+Qed.
+
+Lemma I2F_generate_num_poison_bytes : forall num dt,
+    Forall2 I2F_mbyte
+      (@generate_num_poison_bytes PInf num dt)
+      (@generate_num_poison_bytes PFin num dt).
+Proof.
+  intros; apply I2F_generate_num_poison_bytes_h.
+Qed.
+
+Lemma I2F_generate_poison_bytes : forall dt,
+    Forall2 I2F_mbyte
+      (@generate_poison_bytes PInf dt)
+      (@generate_poison_bytes PFin dt).
+Proof.
+  intros; unfold generate_poison_bytes.
+  rewrite I2F_sizeof_dtyp.
+  apply I2F_generate_num_poison_bytes.
+Qed.
+
+(** * State relation
+
+    Componentwise relation on the concrete implementation's memory
+    state ([State], [Semantics/Implementations/Memory.v]): memories are
+    related as [IM_Refine]-related maps of [I2F_byte]-related bytes,
+    framestacks structurally (so that [pop_frame_stack]'s failure on
+    [Singleton] happens in lockstep), heaps as [IM_Refine]-related maps
+    of [I2F_Addr]-related pointer lists, and provenances *equal*
+    (feeding [Cfresh_prov]'s lockstep resolution and the [aid]/[prov]
+    payloads stored in [I2F_byte]/[I2F_Addr]). *)
+
+Definition I2F_byte (b : @byte PInf) (b' : @byte PFin) : Prop :=
+  let '(mb, aid) := b in
+  let '(mb', aid') := b' in
+  I2F_mbyte mb mb' /\ aid = aid'.
+
+Definition I2F_memory : @memory PInf -> @memory PFin -> Prop := IM_Refine I2F_byte.
+
+Definition I2F_Frame : @Frame PInf -> @Frame PFin -> Prop := Forall2 I2F_Addr.
+
+Inductive I2F_Framestack : @Framestack PInf -> @Framestack PFin -> Prop :=
+| I2F_FS_Singleton f f' : I2F_Frame f f' -> I2F_Framestack (Singleton f) (Singleton f')
+| I2F_FS_Snoc s s' f f' :
+  I2F_Framestack s s' -> I2F_Frame f f' -> I2F_Framestack (Snoc s f) (Snoc s' f')
+.
+
+Definition I2F_Heap : @Heap PInf -> @Heap PFin -> Prop := IM_Refine (Forall2 I2F_Addr).
+
+Record I2F_Memory_stack (ms : @Memory_stack PInf) (ms' : @Memory_stack PFin) : Prop :=
+  { i2f_ms_memory : I2F_memory (Memory_stack_memory ms) (Memory_stack_memory ms');
+    i2f_ms_fs     : I2F_Framestack (Memory_stack_frame_stack ms) (Memory_stack_frame_stack ms');
+    i2f_ms_heap   : I2F_Heap (Memory_stack_heap ms) (Memory_stack_heap ms')
+  }.
+
+Record I2F_State (σ : @State PInf) (σ' : @State PFin) : Prop :=
+  { i2f_st_ms   : I2F_Memory_stack (state_memory_stack σ) (state_memory_stack σ');
+    i2f_st_prov : state_provenance σ = state_provenance σ'
+  }.
+
+(** ** [IM_Refine]/map-operation corollaries *)
+
+Lemma I2F_next_key_with_alignment : forall m1 m2,
+    I2F_memory m1 m2 ->
+    forall align, next_key_with_alignment m1 align = next_key_with_alignment m2 align.
+Proof.
+  intros m1 m2 [DOM _] align.
+  unfold next_key_with_alignment.
+  rewrite (IM_greatest_key_morph _ _ DOM).
+  reflexivity.
+Qed.
+
+Lemma I2F_free_frame_memory : forall f f',
+    I2F_Frame f f' ->
+    forall m1 m2, I2F_memory m1 m2 ->
+    I2F_memory (@free_frame_memory PInf f m1) (@free_frame_memory PFin f' m2).
+Proof.
+  intros f f' HF; induction HF as [| [z pr] [i pr'] fs fs' [HI ->] HF' IH];
+    intros m1 m2 Hm; [cbn; auto|].
+  red in HI; subst.
+  cbn [free_frame_memory fold_left free_byte] in *.
+  apply IH.
+  apply IM_Refine_remove; auto.
+Qed.
+
+Lemma I2F_free_block_memory : forall b b',
+    Forall2 I2F_Addr b b' ->
+    forall m1 m2, I2F_memory m1 m2 ->
+    I2F_memory (@free_block_memory PInf b m1) (@free_block_memory PFin b' m2).
+Proof.
+  intros b b' HB; induction HB as [| [z pr] [i pr'] bs bs' [HI ->] HB' IH];
+    intros m1 m2 Hm; [cbn; auto|].
+  red in HI; subst.
+  cbn [free_block_memory fold_left free_byte] in *.
+  apply IH.
+  apply IM_Refine_remove; auto.
+Qed.
+
+Lemma I2F_add_to_frame : forall ms1 ms2,
+    I2F_Memory_stack ms1 ms2 ->
+    forall (k1 : @ptr (@PROV PInf) (@PTR PInf)) (k2 : @ptr (@PROV PFin) (@PTR PFin)),
+      I2F_Addr k1 k2 ->
+    I2F_Memory_stack (@add_to_frame PInf ms1 k1) (@add_to_frame PFin ms2 k2).
+Proof.
+  intros [m1 s1 h1] [m2 s2 h2] [Hmem Hfs Hheap] k1 k2 Hk; cbn in *.
+  destruct Hfs as [f f' Hf | s s' f f' Hs Hf].
+  - constructor; cbn.
+    + auto.
+    + apply I2F_FS_Singleton; constructor; auto.
+    + auto.
+  - constructor; cbn.
+    + auto.
+    + apply I2F_FS_Snoc; auto; constructor; auto.
+    + auto.
+Qed.
+
+Lemma I2F_add_all_to_frame : forall (ks1 : list (@ptr (@PROV PInf) (@PTR PInf)))
+                                    (ks2 : list (@ptr (@PROV PFin) (@PTR PFin))),
+    Forall2 I2F_Addr ks1 ks2 ->
+    forall ms1 ms2, I2F_Memory_stack ms1 ms2 ->
+    I2F_Memory_stack (@add_all_to_frame PInf ks1 ms1) (@add_all_to_frame PFin ks2 ms2).
+Proof.
+  intros ks1 ks2 HK; induction HK; intros ms1 ms2 Hms; cbn; auto.
+  apply IHHK, I2F_add_to_frame; auto.
+Qed.
+
+Lemma I2F_add_to_heap : forall ms1 ms2,
+    I2F_Memory_stack ms1 ms2 ->
+    forall (root1 : @ptr (@PROV PInf) (@PTR PInf)) (root2 : @ptr (@PROV PFin) (@PTR PFin)),
+      I2F_Addr root1 root2 ->
+    forall (p1 : @ptr (@PROV PInf) (@PTR PInf)) (p2 : @ptr (@PROV PFin) (@PTR PFin)),
+      I2F_Addr p1 p2 ->
+    I2F_Memory_stack (@add_to_heap PInf ms1 root1 p1) (@add_to_heap PFin ms2 root2 p2).
+Proof.
+  intros [m1 s1 h1] [m2 s2 h2] [Hmem Hfs Hheap]
+    [z pr] [i pr'] Hroot p1 p2 Hp; cbn in *.
+  destruct Hroot as [HI ->]; red in HI; subst.
+  unfold add_to_heap, add_with; cbn.
+  constructor.
+  - auto.
+  - auto.
+  - cbn.
+    destruct Hheap as [DOM VAL].
+    lazymatch goal with
+    | |- I2F_Heap match ?e1 with Some _ => _ | None => _ end match ?e2 with Some _ => _ | None => _ end =>
+        destruct e1 as [l1|] eqn:E1; destruct e2 as [l2|] eqn:E2
+    end.
+    + assert (HL : Forall2 I2F_Addr l1 l2) by (eapply VAL; eauto).
+      apply IM_Refine_add; [exact (conj DOM VAL) | constructor; auto].
+    + exfalso.
+      apply lookup_member in E1; apply DOM in E1; apply member_lookup in E1 as [v Hv].
+      assert (Hcontra : Some v = None)
+        by (transitivity (lookup (unsigned i) h2); [symmetry; exact Hv | exact E2]).
+      discriminate.
+    + exfalso.
+      apply lookup_member in E2; apply DOM in E2; apply member_lookup in E2 as [v Hv].
+      assert (Hcontra : Some v = None)
+        by (transitivity (lookup (unsigned i) h1); [symmetry; exact Hv | exact E1]).
+      discriminate.
+    + apply IM_Refine_add; [exact (conj DOM VAL) | constructor; auto].
+Qed.
+
+Lemma I2F_add_all_to_heap' : forall ms1 ms2,
+    I2F_Memory_stack ms1 ms2 ->
+    forall (root1 : @ptr (@PROV PInf) (@PTR PInf)) (root2 : @ptr (@PROV PFin) (@PTR PFin)),
+      I2F_Addr root1 root2 ->
+    forall (ks1 : list (@ptr (@PROV PInf) (@PTR PInf))) (ks2 : list (@ptr (@PROV PFin) (@PTR PFin))),
+      Forall2 I2F_Addr ks1 ks2 ->
+    I2F_Memory_stack (@add_all_to_heap' PInf ms1 root1 ks1) (@add_all_to_heap' PFin ms2 root2 ks2).
+Proof.
+  intros ms1 ms2 Hms root1 root2 Hroot ks1 ks2 HK; revert ms1 ms2 Hms.
+  induction HK; intros ms1 ms2 Hms; cbn; auto.
+  apply IHHK, I2F_add_to_heap; auto.
+Qed.
+
+Lemma I2F_add_all_to_heap : forall (ks1 : list (@ptr (@PROV PInf) (@PTR PInf)))
+                                   (ks2 : list (@ptr (@PROV PFin) (@PTR PFin))),
+    Forall2 I2F_Addr ks1 ks2 ->
+    forall ms1 ms2, I2F_Memory_stack ms1 ms2 ->
+    I2F_Memory_stack (@add_all_to_heap PInf ks1 ms1) (@add_all_to_heap PFin ks2 ms2).
+Proof.
+  intros ks1 ks2 HK; destruct HK as [| k1 k2 ks1 ks2 Hk HK]; intros ms1 ms2 Hms;
+    cbn [add_all_to_heap].
+  - auto.
+  - apply I2F_add_all_to_heap'; auto.
+Qed.
+
+(** ** Accessor pack
+
+    One [I2F_memS]/[I2F_State] lemma per state combinator of
+    [Implementations/Memory.v:403-467]. *)
+
+Lemma I2F_get_mem : I2F_memS I2F_State I2F_memory get_mem get_mem.
+Proof.
+  unfold get_mem.
+  eapply I2F_memS_bind; [apply I2F_memS_get |].
+  intros σ1 σ2 [[Hmem Hfs Hheap] Hprov]; cbn.
+  constructor; exact Hmem.
+Qed.
+
+Lemma I2F_get_frame_stack : I2F_memS I2F_State I2F_Framestack get_frame_stack get_frame_stack.
+Proof.
+  unfold get_frame_stack.
+  eapply I2F_memS_bind; [apply I2F_memS_get |].
+  intros σ1 σ2 [[Hmem Hfs Hheap] Hprov]; cbn.
+  constructor; exact Hfs.
+Qed.
+
+Lemma I2F_get_framestack : I2F_memS I2F_State I2F_Framestack get_framestack get_framestack.
+Proof.
+  unfold get_framestack.
+  eapply I2F_memS_bind; [apply I2F_memS_get |].
+  intros σ1 σ2 [[Hmem Hfs Hheap] Hprov]; cbn.
+  constructor; exact Hfs.
+Qed.
+
+Lemma I2F_get_frame : I2F_memS I2F_State I2F_Frame get_frame get_frame.
+Proof.
+  unfold get_frame.
+  eapply I2F_memS_bind; [apply I2F_get_frame_stack |].
+  intros fs1 fs2 Hfs.
+  destruct Hfs as [f f' Hf | s s' f f' Hs Hf]; constructor; auto.
+Qed.
+
+Lemma I2F_get_heap : I2F_memS I2F_State I2F_Heap get_heap get_heap.
+Proof.
+  unfold get_heap.
+  eapply I2F_memS_bind; [apply I2F_memS_get |].
+  intros σ1 σ2 [[Hmem Hfs Hheap] Hprov]; cbn.
+  constructor; exact Hheap.
+Qed.
+
+Lemma I2F_get_provenance :
+  I2F_memS I2F_State (@Logic.eq provenance) get_provenance get_provenance.
+Proof.
+  unfold get_provenance.
+  eapply I2F_memS_bind; [apply I2F_memS_get |].
+  intros σ1 σ2 [Hms Hprov]; cbn.
+  constructor; exact Hprov.
+Qed.
+
+Lemma I2F_app_mem_stack : forall f1 f2,
+    (forall ms1 ms2, I2F_Memory_stack ms1 ms2 -> I2F_Memory_stack (f1 ms1) (f2 ms2)) ->
+    I2F_memS I2F_State (fun (_ _ : unit) => True) (app_mem_stack f1) (app_mem_stack f2).
+Proof.
+  intros f1 f2 Hf; unfold app_mem_stack.
+  eapply I2F_memS_bind; [apply I2F_memS_get |].
+  intros [ms1 pv1] [ms2 pv2] [Hms Hprov]; cbn in *.
+  apply I2F_memS_put; auto.
+  constructor; cbn; auto.
+Qed.
+
+Lemma I2F_app_mem : forall f1 f2,
+    (forall m1 m2, I2F_memory m1 m2 -> I2F_memory (f1 m1) (f2 m2)) ->
+    I2F_memS I2F_State (fun (_ _ : unit) => True) (app_mem f1) (app_mem f2).
+Proof.
+  intros f1 f2 Hf; unfold app_mem.
+  eapply I2F_memS_bind; [apply I2F_memS_get |].
+  intros [[m1 s1 h1] pv1] [[m2 s2 h2] pv2] [[Hmem Hfs Hheap] Hprov]; cbn in *.
+  apply I2F_memS_put.
+  constructor; cbn.
+  - constructor; cbn; auto.
+  - auto.
+Qed.
+
+Lemma I2F_app_heap : forall f1 f2,
+    (forall h1 h2, I2F_Heap h1 h2 -> I2F_Heap (f1 h1) (f2 h2)) ->
+    I2F_memS I2F_State (fun (_ _ : unit) => True) (app_heap f1) (app_heap f2).
+Proof.
+  intros f1 f2 Hf; unfold app_heap.
+  eapply I2F_memS_bind; [apply I2F_memS_get |].
+  intros [[m1 s1 h1] pv1] [[m2 s2 h2] pv2] [[Hmem Hfs Hheap] Hprov]; cbn in *.
+  apply I2F_memS_put.
+  constructor; cbn.
+  - constructor; cbn; auto.
+  - auto.
+Qed.
+
+Lemma I2F_app_frame_stack : forall f1 f2,
+    (forall fs1 fs2, I2F_Framestack fs1 fs2 -> I2F_Framestack (f1 fs1) (f2 fs2)) ->
+    I2F_memS I2F_State (fun (_ _ : unit) => True) (app_frame_stack f1) (app_frame_stack f2).
+Proof.
+  intros f1 f2 Hf; unfold app_frame_stack.
+  eapply I2F_memS_bind; [apply I2F_memS_get |].
+  intros [[m1 s1 h1] pv1] [[m2 s2 h2] pv2] [[Hmem Hfs Hheap] Hprov]; cbn in *.
+  apply I2F_memS_put.
+  constructor; cbn.
+  - constructor; cbn; auto.
+  - auto.
+Qed.
+
+Lemma I2F_upd_mem : forall m1 m2,
+    I2F_memory m1 m2 ->
+    I2F_memS I2F_State (fun (_ _ : unit) => True) (upd_mem m1) (upd_mem m2).
+Proof. intros; apply I2F_app_mem; auto. Qed.
+
+Lemma I2F_upd_heap : forall h1 h2,
+    I2F_Heap h1 h2 ->
+    I2F_memS I2F_State (fun (_ _ : unit) => True) (upd_heap h1) (upd_heap h2).
+Proof. intros; apply I2F_app_heap; auto. Qed.
+
+Lemma I2F_upd_frame_stack : forall fs1 fs2,
+    I2F_Framestack fs1 fs2 ->
+    I2F_memS I2F_State (fun (_ _ : unit) => True) (upd_frame_stack fs1) (upd_frame_stack fs2).
+Proof. intros; apply I2F_app_frame_stack; auto. Qed.
+
+Lemma I2F_pop_frame_stack : forall fs1 fs2,
+    I2F_Framestack fs1 fs2 ->
+    I2F_EOU I2F_Framestack (pop_frame_stack fs1) (pop_frame_stack fs2).
+Proof.
+  intros fs1 fs2 Hfs; destruct Hfs as [f f' Hf | s s' f f' Hs Hf]; cbn.
+  - constructor.
+  - constructor; auto.
+Qed.
+
+Lemma I2F_app_frame_stack_eob : I2F_memS I2F_State (fun (_ _ : unit) => True)
+    (app_frame_stack_eob pop_frame_stack) (app_frame_stack_eob pop_frame_stack).
+Proof.
+  unfold app_frame_stack_eob.
+  eapply I2F_memS_bind; [apply I2F_get_framestack |].
+  intros fs1 fs2 Hfs.
+  eapply I2F_memS_bind; [apply I2F_memS_lift, I2F_pop_frame_stack; auto |].
+  intros fs1' fs2' Hfs'.
+  apply I2F_upd_frame_stack; auto.
+Qed.
+
+(** ** Primitives
+
+    [Existing Instance MemoryModelPrimitivesV] (declared above) resolves
+    [read_byte]/[write_byte]/[allocate_bytes_with_pr]/[malloc_bytes_with_pr]/
+    [mempush]/[mempop]/[free] to their concrete implementations below. *)
+
+Lemma I2F_read_byte_raw : forall msg addr,
+    I2F_memS I2F_State I2F_byte
+      (read_byte_raw msg addr)
+      (read_byte_raw msg addr).
+Proof.
+  intros msg addr; unfold read_byte_raw, read_byte_raw_mem.
+  eapply I2F_memS_bind; [apply I2F_memS_get |].
+  intros [[m1 s1 h1] pv1] [[m2 s2 h2] pv2] [[Hmem Hfs Hheap] Hprov]; cbn in *.
+  lazymatch goal with
+  | |- I2F_memS I2F_State I2F_byte
+        match ?e1 with Some _ => _ | None => _ end
+        match ?e2 with Some _ => _ | None => _ end =>
+      destruct e1 as [b1|] eqn:E1; destruct e2 as [b2|] eqn:E2
+  end.
+  - constructor; eapply Hmem; eauto.
+  - exfalso.
+    destruct Hmem as [DOM VAL].
+    apply lookup_member in E1; apply DOM in E1; apply member_lookup in E1 as [v Hv].
+    assert (Hcontra : Some v = None)
+      by (transitivity (lookup addr m2); [symmetry; exact Hv | exact E2]).
+    discriminate.
+  - exfalso.
+    destruct Hmem as [DOM VAL].
+    apply lookup_member in E2; apply DOM in E2; apply member_lookup in E2 as [v Hv].
+    assert (Hcontra : Some v = None)
+      by (transitivity (lookup addr m1); [symmetry; exact Hv | exact E1]).
+    discriminate.
+  - constructor.
+Qed.
+
+Lemma I2F_set_byte_raw : forall addr b1 b2,
+    I2F_byte b1 b2 ->
+    I2F_memS I2F_State (fun (_ _ : unit) => True) (set_byte_raw addr b1) (set_byte_raw addr b2).
+Proof.
+  intros addr b1 b2 Hb; unfold set_byte_raw.
+  eapply I2F_memS_bind; [apply I2F_get_mem |].
+  intros m1 m2 Hm.
+  apply I2F_upd_mem.
+  unfold set_byte_raw_mem.
+  apply IM_Refine_add; auto.
+Qed.
+
+Lemma I2F_Read_byte : forall (p1 : @ptr (@PROV PInf) (@PTR PInf)) (p2 : @ptr (@PROV PFin) (@PTR PFin)),
+    I2F_Addr p1 p2 ->
+    I2F_memS I2F_State I2F_mbyte (Read_byte p1) (Read_byte p2).
+Proof.
+  intros [z1 pr1] [z2 pr2] Hp; unfold Read_byte.
+  destruct Hp as [HI ->]; red in HI; subst.
+  eapply I2F_memS_bind; [apply I2F_read_byte_raw |].
+  intros [b1 aid1] [b2 aid2] [Hb Haid]; cbn.
+  rewrite Haid.
+  lazymatch goal with
+  | |- I2F_memS _ _ (if ?c then _ else _) (if ?c then _ else _) => destruct c
+  end.
+  - constructor; auto.
+  - constructor.
+Qed.
+
+Lemma I2F_Write_byte : forall (p1 : @ptr (@PROV PInf) (@PTR PInf)) (p2 : @ptr (@PROV PFin) (@PTR PFin)),
+    I2F_Addr p1 p2 ->
+    forall b1 b2, I2F_mbyte b1 b2 ->
+    I2F_memS I2F_State (fun (_ _ : unit) => True) (Write_byte p1 b1) (Write_byte p2 b2).
+Proof.
+  intros [z1 pr1] [z2 pr2] Hp b1 b2 Hb; unfold Write_byte.
+  destruct Hp as [HI ->]; red in HI; subst.
+  eapply I2F_memS_bind; [apply I2F_read_byte_raw |].
+  intros [b1' aid1] [b2' aid2] [Hb' Haid]; cbn.
+  rewrite Haid.
+  lazymatch goal with
+  | |- I2F_memS _ _ (if ?c then _ else _) (if ?c then _ else _) => destruct c
+  end.
+  - apply I2F_set_byte_raw; split; auto.
+  - constructor.
+Qed.
+
+Lemma I2F_get_free_block : forall size align pr,
+    I2F_memS I2F_State (prod_rel I2F_Addr (Forall2 I2F_Addr))
+      (@get_free_block PInf size align pr) (@get_free_block PFin size align pr).
+Proof.
+  intros size align pr; unfold get_free_block.
+  eapply I2F_memS_bind; [apply I2F_memS_next_key |].
+  intros addr1 addr2 ->.
+  eapply I2F_memS_bind; [apply I2F_memS_lift, I2F_int_to_ptr |].
+  intros ptr1 ptr2 Hptr.
+  eapply I2F_memS_bind; [apply I2F_memS_lift, I2F_get_consecutive_ptrs; auto |].
+  intros ptrs1 ptrs2 Hptrs.
+  constructor; constructor; auto.
+Qed.
+
+Lemma I2F_memory_bytes_to_bytes : forall aid
+    (bytes1 : list (@memory_byte PInf)) (bytes2 : list (@memory_byte PFin)),
+    Forall2 I2F_mbyte bytes1 bytes2 ->
+    Forall2 I2F_byte (@memory_bytes_to_bytes PInf aid bytes1) (@memory_bytes_to_bytes PFin aid bytes2).
+Proof.
+  intros aid bytes1 bytes2 H; induction H; cbn; constructor; auto.
+  split; auto.
+Qed.
+
+Lemma I2F_add_block : forall aid (p1 : @ptr (@PROV PInf) (@PTR PInf)) (p2 : @ptr (@PROV PFin) (@PTR PFin)),
+    I2F_Addr p1 p2 ->
+    forall (ptrs1 : list (@ptr (@PROV PInf) (@PTR PInf))) (ptrs2 : list (@ptr (@PROV PFin) (@PTR PFin)))
+           (bytes1 : list (@memory_byte PInf)) (bytes2 : list (@memory_byte PFin)),
+      Forall2 I2F_mbyte bytes1 bytes2 ->
+    I2F_memS I2F_State (fun (_ _ : unit) => True)
+      (@add_block PInf aid p1 ptrs1 bytes1) (@add_block PFin aid p2 ptrs2 bytes2).
+Proof.
+  intros aid p1 p2 Hp ptrs1 ptrs2 bytes1 bytes2 Hbytes; unfold add_block.
+  destruct p1 as [z1 pr1]; destruct p2 as [z2 pr2].
+  destruct Hp as [HI ->]; red in HI; subst.
+  eapply I2F_memS_bind; [apply I2F_get_mem |].
+  intros m1 m2 Hm.
+  apply I2F_upd_mem.
+  apply IM_Refine_add_all_index; auto.
+  apply I2F_memory_bytes_to_bytes; auto.
+Qed.
+
+Lemma I2F_add_ptrs_to_frame :
+    forall (ptrs1 : list (@ptr (@PROV PInf) (@PTR PInf))) (ptrs2 : list (@ptr (@PROV PFin) (@PTR PFin))),
+    Forall2 I2F_Addr ptrs1 ptrs2 ->
+    I2F_memS I2F_State (fun (_ _ : unit) => True)
+      (@add_ptrs_to_frame PInf ptrs1) (@add_ptrs_to_frame PFin ptrs2).
+Proof.
+  intros ptrs1 ptrs2 Hptrs; unfold add_ptrs_to_frame.
+  apply I2F_app_mem_stack.
+  intros ms1 ms2 Hms; apply I2F_add_all_to_frame; auto.
+Qed.
+
+Lemma I2F_add_ptrs_to_heap :
+    forall (ptrs1 : list (@ptr (@PROV PInf) (@PTR PInf))) (ptrs2 : list (@ptr (@PROV PFin) (@PTR PFin))),
+    Forall2 I2F_Addr ptrs1 ptrs2 ->
+    I2F_memS I2F_State (fun (_ _ : unit) => True)
+      (@add_ptrs_to_heap PInf ptrs1) (@add_ptrs_to_heap PFin ptrs2).
+Proof.
+  intros ptrs1 ptrs2 Hptrs; unfold add_ptrs_to_heap.
+  apply I2F_app_mem_stack.
+  intros ms1 ms2 Hms; apply I2F_add_all_to_heap; auto.
+Qed.
+
+Lemma I2F_add_block_to_stack : forall aid (p1 : @ptr (@PROV PInf) (@PTR PInf)) (p2 : @ptr (@PROV PFin) (@PTR PFin)),
+    I2F_Addr p1 p2 ->
+    forall (ptrs1 : list (@ptr (@PROV PInf) (@PTR PInf))) (ptrs2 : list (@ptr (@PROV PFin) (@PTR PFin))),
+      Forall2 I2F_Addr ptrs1 ptrs2 ->
+    forall (bytes1 : list (@memory_byte PInf)) (bytes2 : list (@memory_byte PFin)),
+      Forall2 I2F_mbyte bytes1 bytes2 ->
+    I2F_memS I2F_State (fun (_ _ : unit) => True)
+      (@add_block_to_stack PInf aid p1 ptrs1 bytes1) (@add_block_to_stack PFin aid p2 ptrs2 bytes2).
+Proof.
+  intros aid p1 p2 Hp ptrs1 ptrs2 Hptrs bytes1 bytes2 Hbytes; unfold add_block_to_stack.
+  eapply I2F_memS_bind; [apply I2F_add_block; auto |].
+  intros _ _ _; apply I2F_add_ptrs_to_frame; auto.
+Qed.
+
+Lemma I2F_add_block_to_heap : forall aid (p1 : @ptr (@PROV PInf) (@PTR PInf)) (p2 : @ptr (@PROV PFin) (@PTR PFin)),
+    I2F_Addr p1 p2 ->
+    forall (ptrs1 : list (@ptr (@PROV PInf) (@PTR PInf))) (ptrs2 : list (@ptr (@PROV PFin) (@PTR PFin))),
+      Forall2 I2F_Addr ptrs1 ptrs2 ->
+    forall (bytes1 : list (@memory_byte PInf)) (bytes2 : list (@memory_byte PFin)),
+      Forall2 I2F_mbyte bytes1 bytes2 ->
+    I2F_memS I2F_State (fun (_ _ : unit) => True)
+      (@add_block_to_heap PInf aid p1 ptrs1 bytes1) (@add_block_to_heap PFin aid p2 ptrs2 bytes2).
+Proof.
+  intros aid p1 p2 Hp ptrs1 ptrs2 Hptrs bytes1 bytes2 Hbytes; unfold add_block_to_heap.
+  eapply I2F_memS_bind; [apply I2F_add_block; auto |].
+  intros _ _ _; apply I2F_add_ptrs_to_heap; auto.
+Qed.
+
+Lemma I2F_Allocate_bytes_with_pr : forall
+    (init_bytes1 : list (@memory_byte PInf)) (init_bytes2 : list (@memory_byte PFin)),
+    Forall2 I2F_mbyte init_bytes1 init_bytes2 ->
+    forall align pr,
+    I2F_memS I2F_State I2F_Addr
+      (@Allocate_bytes_with_pr PInf init_bytes1 align pr)
+      (@Allocate_bytes_with_pr PFin init_bytes2 align pr).
+Proof.
+  intros init_bytes1 init_bytes2 Hbytes align pr; unfold Allocate_bytes_with_pr.
+  rewrite (Forall2_length_N Hbytes).
+  eapply I2F_memS_bind; [apply I2F_get_free_block |].
+  intros [ptr1 ptrs1] [ptr2 ptrs2] [Hptr Hptrs]; cbn in Hptr, Hptrs.
+  eapply I2F_memS_bind; [apply I2F_add_block_to_stack; auto |].
+  intros _ _ _; constructor; auto.
+Qed.
+
+Lemma I2F_Malloc_bytes_with_pr : forall
+    (init_bytes1 : list (@memory_byte PInf)) (init_bytes2 : list (@memory_byte PFin)),
+    Forall2 I2F_mbyte init_bytes1 init_bytes2 ->
+    forall align pr,
+    I2F_memS I2F_State I2F_Addr
+      (@Malloc_bytes_with_pr PInf init_bytes1 align pr)
+      (@Malloc_bytes_with_pr PFin init_bytes2 align pr).
+Proof.
+  intros init_bytes1 init_bytes2 Hbytes align pr; unfold Malloc_bytes_with_pr.
+  rewrite (Forall2_length_N Hbytes).
+  eapply I2F_memS_bind; [apply I2F_get_free_block |].
+  intros [ptr1 ptrs1] [ptr2 ptrs2] [Hptr Hptrs]; cbn in Hptr, Hptrs.
+  eapply I2F_memS_bind; [apply I2F_add_block_to_heap; auto |].
+  intros _ _ _; constructor; auto.
+Qed.
+
+Lemma I2F_push_frame_stack :
+    forall (f1 : @Frame PInf) (f2 : @Frame PFin), I2F_Frame f1 f2 ->
+    forall fs1 fs2, I2F_Framestack fs1 fs2 ->
+    I2F_Framestack (push_frame_stack f1 fs1) (push_frame_stack f2 fs2).
+Proof. intros f1 f2 Hf fs1 fs2 Hfs; constructor; auto. Qed.
+
+Lemma I2F_Mempush : I2F_memS I2F_State (fun (_ _ : unit) => True) Mempush Mempush.
+Proof.
+  unfold Mempush.
+  apply I2F_app_frame_stack.
+  intros fs1 fs2 Hfs; apply I2F_push_frame_stack; auto.
+  constructor.
+Qed.
+
+Lemma I2F_Mempop : I2F_memS I2F_State (fun (_ _ : unit) => True) Mempop Mempop.
+Proof.
+  unfold Mempop.
+  eapply I2F_memS_bind; [apply I2F_get_frame |].
+  intros f1 f2 Hf.
+  eapply I2F_memS_bind; [apply I2F_app_frame_stack_eob |].
+  intros _ _ _.
+  apply I2F_app_mem.
+  intros m1 m2 Hm; apply I2F_free_frame_memory; auto.
+Qed.
+
+Lemma I2F_Free : forall (p1 : @ptr (@PROV PInf) (@PTR PInf)) (p2 : @ptr (@PROV PFin) (@PTR PFin)),
+    I2F_Addr p1 p2 ->
+    I2F_memS I2F_State (fun (_ _ : unit) => True) (Free p1) (Free p2).
+Proof.
+  intros [z1 pr1] [z2 pr2] Hp; unfold Free.
+  destruct Hp as [HI ->]; red in HI; subst.
+  eapply I2F_memS_bind; [apply I2F_get_heap |].
+  intros h1 h2 Hh.
+  destruct Hh as [DOM VAL].
+  lazymatch goal with
+  | |- I2F_memS _ _
+        match ?e1 with Some _ => _ | None => _ end
+        match ?e2 with Some _ => _ | None => _ end =>
+      destruct e1 as [b1|] eqn:E1; destruct e2 as [b2|] eqn:E2
+  end.
+  - assert (HB : Forall2 I2F_Addr b1 b2) by (eapply VAL; eauto).
+    eapply I2F_memS_bind.
+    { apply I2F_app_mem; intros m1 m2 Hm; apply I2F_free_block_memory; auto. }
+    intros _ _ _; apply I2F_upd_heap.
+    apply IM_Refine_remove; exact (conj DOM VAL).
+  - exfalso.
+    apply lookup_member in E1; apply DOM in E1; apply member_lookup in E1 as [v Hv].
+    assert (Hcontra : Some v = None)
+      by (transitivity (lookup (unsigned z2) h2); [symmetry; exact Hv | exact E2]).
+    discriminate.
+  - exfalso.
+    apply lookup_member in E2; apply DOM in E2; apply member_lookup in E2 as [v Hv].
+    assert (Hcontra : Some v = None)
+      by (transitivity (lookup (unsigned z2) h1); [symmetry; exact Hv | exact E1]).
+    discriminate.
+  - constructor.
+Qed.
+
+(** ** Derived operations *)
+
+Lemma I2F_read_bytes : forall (p1 : @ptr (@PROV PInf) (@PTR PInf)) (p2 : @ptr (@PROV PFin) (@PTR PFin)),
+    I2F_Addr p1 p2 -> forall size,
+    I2F_memS I2F_State (Forall2 I2F_mbyte) (read_bytes p1 size) (read_bytes p2 size).
+Proof.
+  intros p1 p2 Hp size; unfold read_bytes.
+  eapply I2F_memS_bind; [apply I2F_memS_lift, I2F_get_consecutive_ptrs; auto |].
+  intros ptrs1 ptrs2 Hptrs.
+  eapply I2F_memS_map_monad_acc2.
+  - exact Hptrs.
+  - intros; apply I2F_Read_byte; auto.
+Qed.
+
+Lemma I2F_read_dvalue : forall (p1 : @ptr (@PROV PInf) (@PTR PInf)) (p2 : @ptr (@PROV PFin) (@PTR PFin)),
+    I2F_Addr p1 p2 -> forall dt,
+    I2F_memS I2F_State I2F_dvalue (read_dvalue dt p1) (read_dvalue dt p2).
+Proof.
+  intros p1 p2 Hp dt; unfold read_dvalue.
+  eapply I2F_memS_bind; [apply I2F_read_bytes; auto |].
+  intros bytes1 bytes2 Hbytes.
+  apply I2F_memS_lift.
+  apply I2F_memory_bytes_to_dvalue; auto.
+Qed.
+
+Lemma Forall2_zip {A1 A2 B1 B2}
+    (RA : A1 -> A2 -> Prop) (RB : B1 -> B2 -> Prop) :
+  forall xs1 xs2, Forall2 RA xs1 xs2 ->
+  forall ys1 ys2, Forall2 RB ys1 ys2 ->
+  Forall2 (prod_rel RA RB) (zip xs1 ys1) (zip xs2 ys2).
+Proof.
+  intros xs1 xs2 Hxs; induction Hxs; intros ys1 ys2 Hys; cbn.
+  - constructor.
+  - destruct Hys; cbn; constructor; auto; constructor; auto.
+Qed.
+
+Lemma I2F_write_bytes : forall (p1 : @ptr (@PROV PInf) (@PTR PInf)) (p2 : @ptr (@PROV PFin) (@PTR PFin)),
+    I2F_Addr p1 p2 ->
+    forall (bytes1 : list (@memory_byte PInf)) (bytes2 : list (@memory_byte PFin)),
+      Forall2 I2F_mbyte bytes1 bytes2 ->
+    I2F_memS I2F_State (fun (_ _ : unit) => True) (write_bytes p1 bytes1) (write_bytes p2 bytes2).
+Proof.
+  intros p1 p2 Hp bytes1 bytes2 Hbytes; unfold write_bytes.
+  rewrite (Forall2_length_N Hbytes).
+  eapply I2F_memS_bind; [apply I2F_memS_lift, I2F_get_consecutive_ptrs; auto |].
+  intros ptrs1 ptrs2 Hptrs.
+  eapply I2F_memS_loop_monad2.
+  - eapply Forall2_zip; eauto.
+  - intros [pa ba] [pb bb] [Hpp Hbb]; cbn; apply I2F_Write_byte; auto.
+Qed.
+
+Lemma I2F_write_dvalue : forall (p1 : @ptr (@PROV PInf) (@PTR PInf)) (p2 : @ptr (@PROV PFin) (@PTR PFin)),
+    I2F_Addr p1 p2 ->
+    forall dt v1 v2, I2F_dvalue v1 v2 ->
+    I2F_memS I2F_State (fun (_ _ : unit) => True) (write_dvalue dt p1 v1) (write_dvalue dt p2 v2).
+Proof.
+  intros p1 p2 Hp dt v1 v2 Hv; unfold write_dvalue.
+  apply I2F_write_bytes; auto.
+  apply I2F_dvalue_to_memory_bytes; auto.
+Qed.
+
+Lemma I2F_allocate_bytes : forall
+    (init_bytes1 : list (@memory_byte PInf)) (init_bytes2 : list (@memory_byte PFin)),
+    Forall2 I2F_mbyte init_bytes1 init_bytes2 ->
+    forall align,
+    I2F_memS I2F_State I2F_Addr
+      (@allocate_bytes PInf _ init_bytes1 align) (@allocate_bytes PFin _ init_bytes2 align).
+Proof.
+  intros init_bytes1 init_bytes2 Hbytes align; unfold allocate_bytes.
+  eapply I2F_memS_bind; [apply I2F_memS_fresh_prov |].
+  intros pr1 pr2 ->.
+  apply I2F_Allocate_bytes_with_pr; auto.
+Qed.
+
+Lemma Forall2_concat {A1 A2} (R : A1 -> A2 -> Prop) :
+  forall ls1 ls2, Forall2 (Forall2 R) ls1 ls2 -> Forall2 R (List.concat ls1) (List.concat ls2).
+Proof.
+  intros ls1 ls2 H; induction H; cbn; auto.
+  apply Forall2_app; auto.
+Qed.
+
+Lemma I2F_allocate_dtyp : forall dt num_elements align,
+    I2F_memS I2F_State I2F_Addr
+      (@allocate_dtyp PInf _ dt num_elements align) (@allocate_dtyp PFin _ dt num_elements align).
+Proof.
+  intros dt num_elements align; unfold allocate_dtyp.
+  destruct (dtyp_eqb dt DTYPE_Void).
+  - constructor.
+  - apply I2F_allocate_bytes.
+    apply Forall2_concat.
+    apply Forall2_repeatN.
+    apply I2F_generate_poison_bytes.
+Qed.
+
+(** ** [convert_impure]: impure type conversions
+
+    [assert_inttoptr_types_ok] is parameter-free (shared [dtyp_base]s);
+    the two arithmetic legs reuse [I2F_dvalue_base_int_unsigned]/
+    [I2F_Addr_ptr_to_int] (equal integer readings of related values) and
+    the already-proved [I2F_int_to_ptr]/[I2F_coerce_integer_to_int]. *)
+
+Lemma I2F_assert_inttoptr_types_ok : forall t_from t_to,
+    I2F_memS I2F_State (fun (_ _ : unit) => True)
+      (@assert_inttoptr_types_ok PInf _ t_from t_to) (@assert_inttoptr_types_ok PFin _ t_from t_to).
+Proof.
+  intros t_from t_to; unfold assert_inttoptr_types_ok.
+  destruct t_from, t_to; constructor; auto.
+Qed.
+
+Lemma I2F_convert_impure_base : forall conv t_from t_to v1 v2,
+    I2F_dvalue_base v1 v2 ->
+    I2F_memS I2F_State I2F_dvalue_base
+      (@convert_impure_base PInf _ conv t_from v1 t_to) (@convert_impure_base PFin _ conv t_from v2 t_to).
+Proof.
+  intros conv t_from t_to v1 v2 Hv; unfold convert_impure_base.
+  destruct conv.
+  - eapply I2F_memS_bind; [apply I2F_assert_inttoptr_types_ok |].
+    intros _ _ _.
+    apply I2F_memS_lift.
+    rewrite (I2F_dvalue_base_int_unsigned Hv).
+    eapply I2F_EOU_bind; [apply I2F_int_to_ptr |].
+    intros a1 a2 Ha; repeat constructor; auto.
+  - destruct Hv as [[z1 pr1] [z2 pr2] HI | | | | | | | ]; [ | constructor .. ].
+    destruct HI as [HI ->]; red in HI; subst.
+    destruct t_to;
+      [ apply I2F_memS_lift; apply I2F_coerce_integer_to_int
+      | apply I2F_memS_lift; apply I2F_coerce_integer_to_int
+      | constructor .. ].
+  - destruct Hv as [[z1 pr1] [z2 pr2] HI | | | | | | | ]; [ | constructor .. ].
+    destruct HI as [HI ->]; red in HI; subst.
+    destruct t_to;
+      [ apply I2F_memS_lift; apply I2F_coerce_integer_to_int
+      | apply I2F_memS_lift; apply I2F_coerce_integer_to_int
+      | constructor .. ].
+  - constructor.
+Qed.
+
+Lemma I2F_convert_impure : forall conv t_from t_to v1 v2,
+    I2F_dvalue v1 v2 ->
+    I2F_memS I2F_State I2F_dvalue
+      (@convert_impure PInf _ conv t_from v1 t_to) (@convert_impure PFin _ conv t_from v2 t_to).
+Proof.
+  intros conv t_from t_to v1 v2 Hv; unfold convert_impure.
+  destruct Hv as [b1 b2 Hb | p s1 s2 Hs | v τ s1 s2 Hs].
+  - destruct (get_base_conversion_type t_from t_to) as [[tf' tt']|]; cbn; [| apply I2F_Merr].
+    eapply I2F_memS_bind; [apply I2F_convert_impure_base; auto |].
+    intros b1' b2' Hb'; apply I2F_Mret; constructor; auto.
+  - cbn; apply I2F_Merr.
+  - destruct v; cbn; [| apply I2F_Merr ..].
+    destruct τ as [ | | vector sz τ]; cbn; [ apply I2F_Merr | apply I2F_Merr | ].
+    destruct vector; cbn; [ | apply I2F_Merr ].
+    destruct (get_vector_conversion_type t_from t_to) as [[tf' tt']|]; cbn; [| apply I2F_Merr].
+    eapply I2F_memS_bind.
+    { apply I2F_memS_lift, I2F_EOU_map_monad2 with (RA := I2F_dvalue); auto.
+      intros a1 a2 Ha; apply I2F_dvalue_to_dvalue_base; auto. }
+    intros elts1' elts2' Helts.
+    eapply I2F_memS_bind.
+    { eapply I2F_memS_map_monad2; eauto.
+      intros x1 x2 Hx; apply I2F_convert_impure_base; auto. }
+    intros val1 val2 Hval.
+    apply I2F_Mret, I2F_dvalue_Array.
+    induction Hval; cbn; constructor; auto.
+Qed.
+
+(** ** [handle_memoryM]
+
+    Case on the two related [MemoryE] events (via [I2FE_Memory]); cross
+    pairs are ruled out by [False], and each diagonal case discharges via
+    the primitive/derived-operation lemmas above, answering per
+    [I2FA_Memory]. *)
+
+Theorem I2F_handle_memoryM :
+  forall T1 T2 (e1 : @MemoryE PInf T1) (e2 : @MemoryE PFin T2),
+    I2FE_Memory e1 e2 ->
+    I2F_memS I2F_State (fun a b => I2FA_Memory e1 a e2 b)
+      (@handle_memoryM PInf _ T1 e1) (@handle_memoryM PFin _ T2 e2).
+Proof.
+  intros T1 T2 e1 e2 H.
+  destruct e1 as [ | | t1 n1 align1 | t1 a1 | t1 a1 v1 | cv1 tf1 v1 tt1];
+    destruct e2 as [ | | t2 n2 align2 | t2 a2 | t2 a2 v2 | cv2 tf2 v2 tt2];
+    simp I2FE_Memory in H; cbn in H; try contradiction; unfold handle_memoryM.
+  - (* MemPush *)
+    eapply I2F_memS_mono; [ | apply I2F_Mempush].
+    intros; simp I2FA_Memory; auto.
+  - (* MemPop *)
+    eapply I2F_memS_mono; [ | apply I2F_Mempop].
+    intros; simp I2FA_Memory; auto.
+  - (* Alloca *)
+    destruct H as [Ht [Hn Halign]]; subst.
+    destruct align2 as [align|]; cbn.
+    all: eapply I2F_memS_bind; [apply I2F_allocate_dtyp |];
+      intros ptr1 ptr2 Hptr;
+      apply I2F_Mret;
+      simp I2FA_Memory;
+      repeat constructor; auto.
+  - (* Load *)
+    destruct H as [Ht Ha]; subst.
+    destruct Ha as [b1 b2 Hb | p1 s1 s2 Hs | v1 τ1 s1 s2 Hs].
+    + destruct Hb as [p1 p2 Hp | | | | | | | ]; [ | apply I2F_Mub_l ..].
+      eapply I2F_memS_mono; [ | apply I2F_read_dvalue; auto].
+      intros; simp I2FA_Memory; auto.
+    + apply I2F_Mub_l.
+    + apply I2F_Mub_l.
+  - (* Store *)
+    destruct H as [Ht [Ha Hv]]; subst.
+    destruct Ha as [b1 b2 Hb | p1 s1 s2 Hs | v1' τ1 s1 s2 Hs].
+    + destruct Hb as [p1 p2 Hp | | | | | | | ]; [ | apply I2F_Mub_l ..].
+      eapply I2F_memS_mono; [ | apply I2F_write_dvalue; auto].
+      intros; simp I2FA_Memory; auto.
+    + apply I2F_Mub_l.
+    + apply I2F_Mub_l.
+  - (* Conv *)
+    destruct H as [Hcv [Htf [Hv Htt]]]; subst.
+    eapply I2F_memS_mono; [ | apply I2F_convert_impure; auto].
+    intros; simp I2FA_Memory; auto.
+Qed.
+
+(** ** [handle_intrinsicM] (memcpy/memset/malloc/free)
+
+    The intrinsic name is shared between the two sides ([I2FE_Intrinsic]
+    forces [f1 = f2]), so the string-based dispatch in [handle_intrinsicM]
+    takes the same branch on both sides; only the memory-touching bodies
+    need relating, reusing the [handle_memoryM] ladder above. *)
+
+Lemma I2F_memcpy : forall (src1 dst1 : @ptr (@PROV PInf) (@PTR PInf))
+                          (src2 dst2 : @ptr (@PROV PFin) (@PTR PFin)),
+    I2F_Addr src1 src2 -> I2F_Addr dst1 dst2 ->
+    forall size volatile,
+    I2F_memS I2F_State (fun (_ _ : unit) => True)
+      (memcpy src1 dst1 size volatile) (memcpy src2 dst2 size volatile).
+Proof.
+  intros src1 dst1 src2 dst2 Hsrc Hdst size volatile.
+  unfold memcpy.
+  rewrite <- (I2F_no_overlap dst1 src1 size dst2 src2 size Hdst Hsrc).
+  rewrite <- (I2F_Addr_ptr_to_int _ _ Hsrc).
+  rewrite <- (I2F_Addr_ptr_to_int _ _ Hdst).
+  destruct (orb (no_overlap dst1 size src1 size) (Z.eqb (ptr_to_int src1) (ptr_to_int dst1))).
+  - eapply I2F_memS_bind; [apply I2F_read_bytes; auto |].
+    intros bytes1 bytes2 Hbytes.
+    apply I2F_write_bytes; auto.
+  - apply I2F_Mub_l.
+Qed.
+
+Lemma I2F_memset : forall (dst1 : @ptr (@PROV PInf) (@PTR PInf)) (dst2 : @ptr (@PROV PFin) (@PTR PFin)),
+    I2F_Addr dst1 dst2 ->
+    forall val len volatile,
+    I2F_memS I2F_State (fun (_ _ : unit) => True)
+      (memset dst1 val len volatile) (memset dst2 val len volatile).
+Proof.
+  intros dst1 dst2 Hdst val len volatile; unfold memset.
+  destruct (Z.ltb len 0); [constructor |].
+  apply I2F_write_bytes; auto.
+  apply Forall2_repeatN.
+  apply I2F_mbyte_MByte; repeat constructor.
+Qed.
+
+Lemma I2F_malloc_bytes : forall
+    (init_bytes1 : list (@memory_byte PInf)) (init_bytes2 : list (@memory_byte PFin)),
+    Forall2 I2F_mbyte init_bytes1 init_bytes2 ->
+    forall align,
+    I2F_memS I2F_State I2F_Addr (malloc_bytes init_bytes1 align) (malloc_bytes init_bytes2 align).
+Proof.
+  intros init_bytes1 init_bytes2 Hbytes align; unfold malloc_bytes.
+  eapply I2F_memS_bind; [apply I2F_memS_fresh_prov |].
+  intros pr1 pr2 ->.
+  apply I2F_Malloc_bytes_with_pr; auto.
+Qed.
+
+Lemma I2F_handle_memcpy : forall (args1 : list (@dvalue_base PInf)) (args2 : list (@dvalue_base PFin)),
+    Forall2 I2F_dvalue_base args1 args2 ->
+    I2F_memS I2F_State (fun (_ _ : unit) => True) (handle_memcpy args1) (handle_memcpy args2).
+Proof.
+  intros args1 args2 Hargs; unfold handle_memcpy.
+  destruct Hargs as [ | dst1 dst2 l1 l2 Hdst Hargs]; [apply I2F_Merr |].
+  destruct Hdst as [pdst1 pdst2 Hpdst | | | | | | | ]; try apply I2F_Merr.
+  destruct Hargs as [ | src1 src2 l1' l2' Hsrc Hargs]; [apply I2F_Merr |].
+  destruct Hsrc as [psrc1 psrc2 Hpsrc | | | | | | | ]; try apply I2F_Merr.
+  destruct Hargs as [ | sz1 sz2 l1'' l2'' Hsz Hargs]; [apply I2F_Merr |].
+  destruct Hsz as [ | szv i1 | ip1 ip2 Hip | | | | | ]; try apply I2F_Merr.
+  - destruct Hargs as [ | vol1 vol2 l1''' l2''' Hvol Hargs]; [apply I2F_Merr |].
+    destruct Hvol as [ | szv2 vv1 | | | | | | ]; try apply I2F_Merr.
+    destruct Hargs; [ | apply I2F_Merr].
+    apply I2F_memcpy; auto.
+  - destruct Hargs as [ | vol1 vol2 l1''' l2''' Hvol Hargs]; [apply I2F_Merr |].
+    destruct Hvol as [ | szv2 vv1 | | | | | | ]; try apply I2F_Merr.
+    destruct Hargs; [ | apply I2F_Merr].
+    red in Hip; subst; cbn.
+    apply I2F_memcpy; auto.
+Qed.
+
+Lemma I2F_handle_memset : forall (args1 : list (@dvalue_base PInf)) (args2 : list (@dvalue_base PFin)),
+    Forall2 I2F_dvalue_base args1 args2 ->
+    I2F_memS I2F_State (fun (_ _ : unit) => True) (handle_memset args1) (handle_memset args2).
+Proof.
+  intros args1 args2 Hargs; unfold handle_memset.
+  destruct Hargs as [ | dst1 dst2 l1 l2 Hdst Hargs]; [apply I2F_Merr |].
+  destruct Hdst as [pdst1 pdst2 Hpdst | | | | | | | ]; try apply I2F_Merr.
+  destruct Hargs as [ | val1 val2 l1' l2' Hval Hargs]; [apply I2F_Merr |].
+  destruct Hval as [ | szval v1 | | | | | | ]; try apply I2F_Merr.
+  destruct Hargs as [ | len1 len2 l1'' l2'' Hlen Hargs]; [apply I2F_Merr |].
+  destruct Hlen as [ | szlen ln1 | | | | | | ]; try apply I2F_Merr.
+  destruct Hargs as [ | vol1 vol2 l1''' l2''' Hvol Hargs]; [apply I2F_Merr |].
+  destruct Hvol as [ | szvol vv1 | | | | | | ]; try apply I2F_Merr.
+  destruct Hargs; [ | apply I2F_Merr].
+  destruct (Pos.eq_dec szval 8) as [e | ]; [ | apply I2F_Merr].
+  subst; cbn.
+  apply I2F_memset; auto.
+Qed.
+
+Lemma I2F_handle_malloc : forall (args1 : list (@dvalue_base PInf)) (args2 : list (@dvalue_base PFin)),
+    Forall2 I2F_dvalue_base args1 args2 ->
+    forall align,
+    I2F_memS I2F_State I2F_Addr (handle_malloc args1 align) (handle_malloc args2 align).
+Proof.
+  intros args1 args2 Hargs align; unfold handle_malloc.
+  destruct Hargs as [ | sz1 sz2 l1 l2 Hsz Hargs]; [apply I2F_Merr |].
+  destruct Hsz as [ | szv i1 | ip1 ip2 Hip | | | | | ]; try (destruct Hargs; apply I2F_Merr).
+  - destruct Hargs; [ | apply I2F_Merr].
+    apply I2F_malloc_bytes, I2F_generate_num_poison_bytes.
+  - destruct Hargs; [ | apply I2F_Merr].
+    red in Hip; subst; cbn.
+    apply I2F_malloc_bytes, I2F_generate_num_poison_bytes.
+Qed.
+
+Lemma I2F_handle_free : forall (args1 : list (@dvalue_base PInf)) (args2 : list (@dvalue_base PFin)),
+    Forall2 I2F_dvalue_base args1 args2 ->
+    I2F_memS I2F_State (fun (_ _ : unit) => True) (handle_free args1) (handle_free args2).
+Proof.
+  intros args1 args2 Hargs; unfold handle_free.
+  destruct Hargs as [ | p1 p2 l1 l2 Hp Hargs]; [apply I2F_Merr |].
+  destruct Hp as [pdst1 pdst2 Hpdst | | | | | | | ]; try apply I2F_Merr.
+  destruct Hargs; [ | apply I2F_Merr].
+  apply I2F_Free; auto.
+Qed.
+
+Theorem I2F_handle_intrinsicM :
+  forall T1 T2 (e1 : @IntrinsicE PInf T1) (e2 : @IntrinsicE PFin T2),
+    I2FE_Intrinsic e1 e2 ->
+    I2F_memS I2F_State (fun a b => I2FA_Intrinsic e1 a e2 b)
+      (@handle_intrinsicM PInf _ T1 e1) (@handle_intrinsicM PFin _ T2 e2).
+Proof.
+  intros T1 T2 e1 e2 H.
+  destruct e1 as [t1 f1 args1 va1]; destruct e2 as [t2 f2 args2 va2].
+  simp I2FE_Intrinsic in H; cbn in H.
+  destruct H as [Ht [Hf [Hargs Hva]]]; subst.
+  unfold handle_intrinsicM.
+  eapply I2F_memS_bind.
+  { apply I2F_memS_lift.
+    eapply I2F_EOU_map_monad2; [exact Hargs |].
+    intros a1 a2 Ha; apply I2F_dvalue_to_dvalue_base; auto. }
+  intros args1' args2' Hargs'.
+  destruct (orb (Rocqlib.proj_sumbool (string_dec f2 "llvm.memcpy.p0i8.p0i8.i32"))
+              (Rocqlib.proj_sumbool (string_dec f2 "llvm.memcpy.p0i8.p0i8.i64"))).
+  - eapply I2F_memS_bind; [apply I2F_handle_memcpy; auto |].
+    intros _ _ _; apply I2F_Mret; simp I2FA_Intrinsic; repeat constructor.
+  - destruct (orb (Rocqlib.proj_sumbool (string_dec f2 "llvm.memset.p0i8.i32"))
+                (Rocqlib.proj_sumbool (string_dec f2 "llvm.memset.p0i8.i64"))).
+    + eapply I2F_memS_bind; [apply I2F_handle_memset; auto |].
+      intros _ _ _; apply I2F_Mret; simp I2FA_Intrinsic; repeat constructor.
+    + destruct (Rocqlib.proj_sumbool (string_dec f2 "malloc")).
+      * eapply I2F_memS_bind; [apply I2F_handle_malloc; auto |].
+        intros ptr1 ptr2 Hptr; apply I2F_Mret; simp I2FA_Intrinsic; repeat constructor; auto.
+      * destruct (Rocqlib.proj_sumbool (string_dec f2 "free")).
+        -- eapply I2F_memS_bind; [apply I2F_handle_free; auto |].
+           intros _ _ _; apply I2F_Mret; simp I2FA_Intrinsic; repeat constructor.
+        -- apply I2F_Merr.
+Qed.
