src/rocq/Theory/I2F/I2F_toplevel.v
@@ -1,0 +1,440 @@
+From Equations Require Import Equations.
+
+From Stdlib Require Import
+  ZArith
+  Strings.String
+  List.
+Import ListNotations.
+
+From ITree Require Import Basics.HeterogeneousRelations ITree.
+From ExtLib Require Import Structures.Maps.
+
+From Vellvm Require Import
+  Utils
+  Syntax
+  Semantics
+  VellvmIntegers
+  Integers
+  Interfaces.IPtr
+  Interfaces.Params
+  Interfaces.Pointer
+  Implementations.Pointer
+  Implementations.Provenance
+  Implementations.IPtrInfinite
+  Implementations.IPtrFinite
+  Implementations.Memory
+  Implementations.ParamsV
+  Interfaces.Memory.
+
+From Vellvm Require Import
+  Handlers
+  Semantics.InterpretationStack
+  Semantics.TopLevel
+  Semantics.Libraries
+  Utils.rutt_cutoff.
+
+From Vellvm Require Import
+  Theory.I2F.Refinement
+  Theory.I2F.I2F_exp
+  Theory.I2F.I2F_denotation
+  Theory.I2F.I2F_MemS
+  Theory.I2F.I2F_memory
+  Theory.I2F.I2F_state.
+
+Existing Instance MemoryModelStateV.
+Existing Instance MemoryModelPrimitivesV.
+
+(** * Lifting the interpreter-level result ([I2F_interp_mcfg], [I2F_state.v]) to the top level. *)
+
+(** ** Initial state *)
+Lemma I2F_initial_FusedS :
+  I2F_FusedS
+    (initial_state, ((Build_stack_frame Maps.empty None None, []), Maps.empty))
+    (initial_state, ((Build_stack_frame Maps.empty None None, []), Maps.empty)).
+Proof.
+  constructor; cbn.
+  - constructor; cbn.
+    + constructor; cbn.
+      * apply IM_Refine_empty.
+      * constructor; constructor.
+      * apply IM_Refine_empty.
+    + cbn; reflexivity.
+  - constructor; cbn.
+    + apply RM_Refine_empty.
+    + constructor.
+    + reflexivity.
+  - constructor.
+  - apply RM_Refine_empty.
+Qed.
+
+(** ** Global environment construction *)
+
+Lemma I2F_allocate_global : forall (g : global dtyp),
+    I2F_refine_MCFG (fun (_ _ : unit) => True)
+      (@allocate_global PInf g) (@allocate_global PFin g).
+Proof.
+  intros g; unfold allocate_global.
+  destruct (g_alias g).
+  - apply ruttc_ret; auto.
+  - rbind I2F_dvalue.
+    + unfold alloca; rstep.
+    + intros v1 v2 Hv; unfold gwrite; rstep.
+Qed.
+
+Lemma I2F_allocate_globals : forall (gs : list (global dtyp)),
+    I2F_refine_MCFG (fun (_ _ : unit) => True)
+      (@allocate_globals PInf gs) (@allocate_globals PFin gs).
+Proof.
+  intros gs; unfold allocate_globals, loop_monad.
+  induction gs as [| g gs' IH]; cbn.
+  - apply ruttc_ret; auto.
+  - rbind (fun (_ _ : unit) => True); [apply I2F_allocate_global | intros [] [] _; apply IH].
+Qed.
+
+Lemma I2F_allocate_declaration : forall (d : declaration dtyp),
+    I2F_refine_MCFG (fun (_ _ : unit) => True)
+      (@allocate_declaration PInf d) (@allocate_declaration PFin d).
+Proof.
+  intros d; unfold allocate_declaration.
+  destruct (lookup_intrinsic_declaration (dc_name d)).
+  - apply ruttc_ret; auto.
+  - rbind I2F_dvalue.
+    + unfold alloca; rstep.
+    + intros v1 v2 Hv; unfold gwrite; rstep.
+Qed.
+
+Lemma I2F_allocate_declarations : forall (ds : list (declaration dtyp)),
+    I2F_refine_MCFG (fun (_ _ : unit) => True)
+      (@allocate_declarations PInf ds) (@allocate_declarations PFin ds).
+Proof.
+  intros ds; unfold allocate_declarations, loop_monad.
+  induction ds as [| d ds' IH]; cbn.
+  - apply ruttc_ret; auto.
+  - rbind (fun (_ _ : unit) => True); [apply I2F_allocate_declaration | intros [] [] _; apply IH].
+Qed.
+
+Lemma I2F_initialize_global : forall (g : global dtyp),
+    I2F_refine_MCFG (fun (_ _ : unit) => True)
+      (@initialize_global PInf g) (@initialize_global PFin g).
+Proof.
+  intros g; unfold initialize_global.
+  destruct (g_alias g).
+  - destruct (g_exp g) as [e|].
+    + destruct e; try (apply ruttc_trigger_cast; cbnn; simp I2FE_UB; auto).
+      destruct id; try (apply ruttc_trigger_cast; cbnn; simp I2FE_UB; auto).
+      rbind I2F_dvalue.
+      * unfold gread; rstep.
+      * intros p1 p2 Hp; unfold gwrite; rstep.
+    + apply ruttc_trigger_cast; cbnn; simp I2FE_UB; auto.
+  - rbind I2F_dvalue.
+    + unfold gread; rstep.
+    + intros a1 a2 Ha.
+      rbind I2F_dvalue.
+      * destruct (g_exp g).
+        -- apply I2F_denote_exp.
+        -- apply ruttc_ret; repeat constructor.
+      * intros uv1 uv2 Huv; unfold store; rstep.
+Qed.
+
+Lemma I2F_initialize_globals : forall (gs : list (global dtyp)),
+    I2F_refine_MCFG (fun (_ _ : unit) => True)
+      (@initialize_globals PInf gs) (@initialize_globals PFin gs).
+Proof.
+  intros gs; unfold initialize_globals, loop_monad.
+  induction gs as [| g gs' IH]; cbn.
+  - apply ruttc_ret; auto.
+  - rbind (fun (_ _ : unit) => True); [apply I2F_initialize_global | intros [] [] _; apply IH].
+Qed.
+
+Lemma I2F_build_global_environment : forall (mcfg : CFG.mcfg dtyp),
+    I2F_refine_MCFG (fun (_ _ : unit) => True)
+      (@build_global_environment PInf mcfg) (@build_global_environment PFin mcfg).
+Proof.
+  intros mcfg; unfold build_global_environment.
+  rbind (fun (_ _ : unit) => True).
+  - apply I2F_allocate_declarations.
+  - intros [] [] _.
+    rbind (fun (_ _ : unit) => True).
+    + apply I2F_allocate_globals.
+    + intros [] [] _; apply I2F_initialize_globals.
+Qed.
+
+(** ** Command-line argument allocation *)
+
+Lemma I2F_i8_array_of_string : forall (s : string),
+    I2F_dvalue (@i8_array_of_string PInf s) (@i8_array_of_string PFin s).
+Proof.
+  intros s; unfold i8_array_of_string.
+  constructor.
+  apply Forall2_app.
+  - apply Forall2_map2; intros; repeat constructor.
+  - repeat constructor.
+Qed.
+
+Lemma I2F_allocate_arg : forall (arg : string),
+    I2F_refine_MCFG I2F_dvalue
+      (@allocate_arg PInf arg) (@allocate_arg PFin arg).
+Proof.
+  intros arg; unfold allocate_arg.
+  pose proof (I2F_i8_array_of_string arg) as Harr.
+  rbind I2F_dvalue.
+  - unfold alloca; rstep.
+  - intros v1 v2 Hv.
+    rbind (fun (_ _ : unit) => True).
+    + unfold store.
+      apply ruttc_trigger;
+        [cbnn; simp I2FE_Memory; auto | intros [] [] _; auto].
+    + intros [] [] _; apply ruttc_ret; auto.
+Qed.
+
+Lemma I2F_allocate_args : forall (args : list string),
+    I2F_refine_MCFG I2F_dvalue
+      (@allocate_args PInf args) (@allocate_args PFin args).
+Proof.
+  intros args; unfold allocate_args.
+  rbind I2F_dvalue.
+  - unfold alloca; rstep.
+  - intros v1 v2 Hv.
+    rbind (Forall2 I2F_dvalue).
+    + apply ruttc_map_monad; intros; apply I2F_allocate_arg.
+    + intros addrs1 addrs2 Haddrs.
+      rbind (fun (_ _ : unit) => True).
+      * unfold store.
+        apply ruttc_trigger;
+          [cbnn; simp I2FE_Memory; auto | intros [] [] _; auto].
+      * intros [] [] _; apply ruttc_ret; auto.
+Qed.
+
+Lemma I2F_build_main_args : forall (args : list string),
+    I2F_refine_MCFG (Forall2 I2F_dvalue)
+      (@build_main_args PInf args) (@build_main_args PFin args).
+Proof.
+  intros args; unfold build_main_args.
+  rbind I2F_dvalue; [apply I2F_allocate_args | ].
+  intros v1 v2 Hv; apply ruttc_ret.
+  repeat constructor; auto.
+Qed.
+
+(** ** Function table construction *)
+
+Lemma I2F_address_one_function : forall (df : definition dtyp (CFG.cfg dtyp)),
+    I2F_refine_MCFG (prod_rel Logic.eq I2F_function_denotation)
+      (@address_one_function PInf df) (@address_one_function PFin df).
+Proof.
+  intros df; unfold address_one_function.
+  rbind I2F_dvalue.
+  - unfold gread; rstep.
+  - intros fv1 fv2 Hfv.
+    destruct Hfv as [b1 b2 Hb | | ];
+      try (apply ruttc_trigger_cast; cbnn; simp I2FE_Failure; auto).
+    destruct Hb; try (apply ruttc_trigger_cast; cbnn; simp I2FE_Failure; auto).
+    apply ruttc_ret.
+    constructor; cbn.
+    + apply I2F_Addr_ptr_to_int; auto.
+    + apply I2F_denote_function.
+Qed.
+
+Lemma I2F_address_one_library_function :
+  forall (fid : function_id) (d1 : @function_denotation PInf) (d2 : @function_denotation PFin),
+    I2F_function_denotation d1 d2 ->
+    I2F_refine_MCFG (prod_rel Logic.eq I2F_function_denotation)
+      (@address_one_library_function PInf (fid, d1))
+      (@address_one_library_function PFin (fid, d2)).
+Proof.
+  intros fid d1 d2 Hd; unfold address_one_library_function.
+  rbind I2F_dvalue.
+  - unfold gread; rstep.
+  - intros fv1 fv2 Hfv.
+    destruct Hfv as [b1 b2 Hb | | ];
+      try (apply ruttc_trigger_cast; cbnn; simp I2FE_Failure; auto).
+    destruct Hb; try (apply ruttc_trigger_cast; cbnn; simp I2FE_Failure; auto).
+    apply ruttc_ret.
+    constructor; cbn; auto.
+    apply I2F_Addr_ptr_to_int; auto.
+Qed.
+
+(** The built-in library denotations themselves *)
+#[local] Arguments Pos.eq_dec : simpl never.
+
+Lemma I2F_putchar_denotation :
+  I2F_function_denotation (@putchar_denotation PInf) (@putchar_denotation PFin).
+Proof.
+  intros args1 args2 Hargs.
+  unfold putchar_denotation; cbn.
+  destruct Hargs as [| u1 u2 args1 args2 Hu Hargs]; [apply ruttc_trigger_cast; cbnn; simp I2FE_Failure; auto|].
+  destruct Hargs; cbn; [ | unfold raise; apply ruttc_trigger_cast; cbnn; simp I2FE_Failure; auto].
+  unfold ITree.map.
+  destruct Hu as [b1 b2 Hb | | ]; try (rbind (fun _ _ => False); [apply ruttc_trigger_cast; cbnn; simp I2FE_UB; auto | intros ?? []]); [].
+  destruct Hb as [p1 p2 Hp | sz i | p1 p2 Hp | d | f | t | | sz bits1 bits2 Hbits]; try (rbind (fun _ _ => False); [apply ruttc_trigger_cast; cbnn; simp I2FE_UB; auto | intros ?? []]); [].
+  destruct (Pos.eq_dec 32 sz); cbn.
+  - rewrite 2 Eqit.bind_bind.
+    rbind TT; [rstep | intros [] [] _].
+    rewrite 2 Eqit.bind_ret_l; rstep.
+  - try (rbind (fun _ _ => False); [apply ruttc_trigger_cast; cbnn; simp I2FE_UB; auto | intros ?? []]).
+Qed.
+
+Lemma I2F_i8_str_index :
+  forall (p1 : @ptr (@PROV PInf) (@PTR PInf)) (p2 : @ptr (@PROV PFin) (@PTR PFin))
+    (index : Z),
+    I2F_Addr p1 p2 ->
+    I2F_refine_CFG Logic.eq
+      (@i8_str_index PInf p1 index) (@i8_str_index PFin p2 index).
+Proof.
+  intros p1 p2 index Hp.
+  unfold i8_str_index.
+  rbind I2F_Iptr.
+  - apply I2F_refine_lift', I2F_from_Z.
+  - intros iptr1 iptr2 Hiptr.
+    rbind I2F_Addr.
+    + apply I2F_refine_lift', I2F_handle_gep_ptr; auto.
+    + intros addr1 addr2 Haddr.
+      rbind I2F_dvalue.
+      * unfold load.
+        apply ruttc_trigger;
+          [cbnn; simp I2FE_Memory; auto | intros a b Hab; cbnn in Hab; simp I2FA_Memory in Hab; auto].
+      * intros d1 d2 Hd.
+        destruct Hd as [b1 b2 Hb | | ];
+          try (unfold raise; apply ruttc_trigger_cast; cbnn; simp I2FE_Failure; auto); [].
+        destruct Hb as [q1 q2 Hq | sz i | q1 q2 Hq | dd | ff | tt | | sz bits1 bits2 Hbits];
+          try (unfold raise; apply ruttc_trigger_cast; cbnn; simp I2FE_Failure; auto); [].
+        repeat (destruct sz as [sz|sz|]; cbn;
+          try (apply ruttc_trigger_cast; cbnn; simp I2FE_Failure; auto)).
+        apply ruttc_ret; auto.
+Qed.
+
+#[local] Arguments Integers.eq : simpl never.
+Lemma I2F_puts_denotation :
+  I2F_function_denotation (@puts_denotation PInf) (@puts_denotation PFin).
+Proof.
+  intros args1 args2 Hargs.
+  unfold puts_denotation.
+  destruct Hargs as [| u1 u2 args1 args2 Hu Hargs];
+    [apply ruttc_trigger_cast; cbnn; simp I2FE_Failure; auto|].
+  destruct Hargs; [ | unfold raise; apply ruttc_trigger_cast; cbnn; simp I2FE_Failure; auto].
+  destruct Hu as [b1 b2 Hb | | ];
+    try (rbind (fun _ _ => False); [apply ruttc_trigger_cast; cbnn; simp I2FE_UB; auto | intros ?? []]); [].
+  destruct Hb as [p1 p2 Hp | sz i | p1 p2 Hp | d | f | t | | sz bits1 bits2 Hbits];
+    try (rbind (fun _ _ => False); [apply ruttc_trigger_cast; cbnn; simp I2FE_UB; auto | intros ?? []]); [].
+  simpl; unfold ITree.map.
+  rewrite !Eqit.bind_bind.
+  rbind Logic.eq.
+  - apply I2F_i8_str_index; auto.
+  - intros c1 c2 <-.
+    rewrite !Eqit.bind_bind.
+    rbind Logic.eq.
+    + apply ruttc_iter with (II := Logic.eq).
+      * intros [[c1' bytes1] off1] ? <-.
+        break_match_goal; [rstep |].
+        rbind Logic.eq.
+        apply I2F_i8_str_index; auto.
+        intros nc1 nc2 <-; rstep.
+      * reflexivity.
+    + intros bytes1 bytes2 <-.
+      rewrite !Eqit.bind_bind.
+      rbind (fun (_ _ : unit) => True).
+      * apply ruttc_trigger; [cbnn; simp I2FE_ExternalCall; auto | intros [] [] _; auto].
+      * intros [] [] _.
+        rewrite !Eqit.bind_ret_l; rstep.
+Qed.
+
+Lemma I2F_LIBRARIES :
+  Forall2 (prod_rel Logic.eq I2F_function_denotation)
+    (@_LIBRARIES PInf) (@_LIBRARIES PFin).
+Proof.
+  unfold _LIBRARIES.
+  constructor; [constructor; [reflexivity | apply I2F_puts_denotation] |].
+  constructor; [constructor; [reflexivity | apply I2F_putchar_denotation] |].
+  constructor.
+Qed.
+
+Lemma I2F_library_functions : forall (decls : list (declaration dtyp)),
+    Forall2 (prod_rel Logic.eq I2F_function_denotation)
+      (@library_functions PInf decls) (@library_functions PFin decls).
+Proof.
+  intros decls; unfold library_functions.
+  apply Forall2_filter.
+  - intros [n1 d1] [n2 d2] [Heq _]; cbn in Heq; subst; reflexivity.
+  - apply I2F_LIBRARIES.
+Qed.
+
+(** Turning a [Forall2 (eq × I2F_function_denotation)]-related pair of
+    association lists into an [I2F_ctx]-related pair of [IntMap]s. *)
+Lemma I2F_ctx_of_list :
+  forall (l1 : list (Z * @function_denotation PInf))
+    (l2 : list (Z * @function_denotation PFin)),
+    Forall2 (prod_rel Logic.eq I2F_function_denotation) l1 l2 ->
+    I2F_ctx (IP.of_list l1) (IP.of_list l2).
+Proof.
+  intros l1 l2 H k.
+  apply IM_Refine_lookup, IM_Refine_Forall2; auto.
+Qed.
+
+(** ** [denote_vellvm] ([TopLevel.v:273-286])
+
+    Glues [build_global_environment], the [defns]/[libraries] function
+    table (via [address_one_function]/[address_one_library_function]/
+    [I2F_ctx_of_list]), the final [gread entry], [I2F_denote_mcfg]
+    ([I2F_denotation.v]) on the resulting [I2F_ctx]/[I2F_dvalue]-related
+    address and args, and the closing [match] on the [exc + dvalue]
+    result (([inl],[inl]) via [raiseLLVM]/[I2FE_Exc]-triggering,
+    ([inr],[inr]) via [ret]). *)
+Lemma I2F_denote_vellvm :
+  forall (ret_typ : dtyp) (entry : function_id)
+    (args1 : list (@dvalue PInf)) (args2 : list (@dvalue PFin))
+    (mcfg : CFG.mcfg dtyp),
+    Forall2 I2F_dvalue args1 args2 ->
+    I2F_refine_MCFG I2F_dvalue
+      (@denote_vellvm PInf ret_typ entry args1 mcfg)
+      (@denote_vellvm PFin ret_typ entry args2 mcfg).
+Proof.
+  intros * HDV.
+  unfold denote_vellvm.
+  erbind; [apply I2F_build_global_environment | intros [] [] _].
+  erbind; [apply ruttc_map_monad; intros; apply I2F_address_one_function | intros].
+  erbind. apply ruttc_map_monad_gen.
+  - induction (I2F_library_functions (m_declarations mcfg))
+      as [| [fid1 d1] [fid2 d2] l1 l2 [Heq Hd] Hrest IH].
+    + constructor.
+    + cbn in Heq; subst.
+      constructor; [apply I2F_address_one_library_function; auto | apply IH].
+  - intros libs1 libs2 Hlibs.
+    rbind I2F_dvalue.
+    + unfold gread; rstep.
+    + intros addr1 addr2 Haddr.
+      rbind (sum_rel I2F_dvalue I2F_dvalue).
+      * apply I2F_denote_mcfg; [auto | auto | apply I2F_ctx_of_list, Forall2_app; auto].
+      * intros rv1 rv2 Hrv.
+        destruct Hrv as [exc1 exc2 Hexc | v1 v2 Hv].
+        -- apply ruttc_trigger_cast; cbnn; simp I2FE_Exc; auto.
+        -- apply ruttc_ret; auto.
+Qed.
+
+(** ** [interpreter_gen] / [interpreter_param]
+    The final assembly. *)
+Lemma I2F_interpreter_gen :
+  forall (ret_typ : dtyp) (entry : function_id)
+    (arg_gen1 : @MCFGtop PInf (list (@dvalue PInf)))
+    (arg_gen2 : @MCFGtop PFin (list (@dvalue PFin)))
+    (prog : ll_toplevel_entities),
+    I2F_refine_MCFG (Forall2 I2F_dvalue) arg_gen1 arg_gen2 ->
+    I2F_refine_MCFGbot (prod_rel I2F_FusedS I2F_dvalue)
+      (@interpreter_gen PInf ret_typ entry arg_gen1 prog)
+      (@interpreter_gen PFin ret_typ entry arg_gen2 prog).
+Proof.
+  intros.
+  unfold interpreter_gen.
+  eapply I2F_interp_mcfg_bind; eauto; cycle -1.
+  { apply I2F_initial_FusedS. }
+  intros.
+  now apply I2F_denote_vellvm.
+Qed.
+  
+Theorem I2F_interpreter_param :
+  forall (args : list string) (prog : ll_toplevel_entities),
+    I2F_refine_MCFGbot (prod_rel I2F_FusedS I2F_dvalue)
+      (@interpreter_param PInf args prog)
+      (@interpreter_param PFin args prog).
+Proof.
+  intros.
+  apply I2F_interpreter_gen, I2F_build_main_args.
+Qed.
